theories/adequacy.v
@@ -1,6 +1,29 @@
 From Paco Require Import paco.
 
-From stbor Require Import simulation.
+From stbor Require Import simulation steps_wf.
+
+(** Behaviors ----------------------------------------------------------------*)
+
+Inductive behavior := | Term (v: val) | Stuck | Diverges.
+
+Inductive behaviors
+  (step: expr * config → expr * config → Prop)
+  (cfg: expr * config) : behavior → Prop :=
+| behaviors_term v
+    (TERMINAL: to_val cfg.1 = Some v) :
+    behaviors step cfg (Term v)
+| behaviors_stuck
+    (NT: ¬ terminal cfg.1)
+    (NS: ∀ cfg', ¬ step cfg cfg') :
+    behaviors step cfg Stuck
+(* | behaviors_diverges
+    (DIV: diverges step cfg) :
+    behaviors step cfg Diverges *)
+| behaviors_step cfg' ov
+    (STEP: step cfg cfg')
+    (NEXT: behaviors step cfg' ov):
+    behaviors step cfg ov
+.
 
 (* If c1 ->* c2 -b-> v then c1 -b-> v *)
 Lemma rtc_step_behavior step c1 c2 v
@@ -8,41 +31,38 @@ Lemma rtc_step_behavior step c1 c2 v
   behaviors step c1 v.
 Proof.
   induction STEPS as [|c1 c2 c3 S1 S2 IH]; [done|]. specialize (IH BEH).
-  econstructor 4; eauto.
+  econstructor 3; eauto.
 Qed.
 
-Lemma sim_adequacy {A: Type} Φ (sim_mem: A → state → state → Prop)
-  (σG: A) (cfg_src cfg_tgt: expr * state)
-  (WFS: Wf cfg_src.2) (WFT: Wf cfg_tgt.2)
-  (SIM0: sim_state sim_mem σG cfg_src.2 cfg_tgt.2)
-  (NO_UB: ∀ cfg', cfg_src ~t~>* cfg' → ¬ stuck cfg'.1 cfg'.2)
-  (SIM: @sim A Φ sim_mem σG cfg_src cfg_tgt) :
+Lemma sim_adequacy (cfg_src cfg_tgt: expr * config)
+  (WFS: Wf cfg_src.2) (WFT: Wf cfg_tgt.2) (NO_UB: no_UB cfg_src)
+  (SIM: sim cfg_src cfg_tgt) :
   behaviors tstep cfg_tgt <1= behaviors tstep cfg_src.
 Proof.
-  intros ov BEH. revert σG cfg_src WFS WFT SIM0 NO_UB SIM.
-  induction BEH as [cfg_tgt|cfg_tgt|cfg_tgt v|cfg_tgt cfg_tgt' ov STEP BEH IH];
-    intros σG cfg_src WFS WFT SIM0 NO_UB SIM.
-  - punfold SIM. destruct (SIM WFS WFT SIM0) as (? & ? & TERM & ?); [naive_solver|].
-    destruct TERM as (eσ2 & σG' & TS & TERM' & VAL); [by eexists|].
+  intros ov BEH. revert cfg_src WFS WFT NO_UB SIM.
+  induction BEH as [cfg_tgt(* |cfg_tgt *)|cfg_tgt v|cfg_tgt cfg_tgt' ov STEP BEH IH];
+    intros cfg_src WFS WFT NO_UB SIM.
+  - punfold SIM. destruct (SIM WFS WFT) as [? (* ? *) TERM ?]; [naive_solver|].
+    destruct TERM as (eσ2 & TS & TERM' & VAL); [by eexists|].
     apply (rtc_step_behavior _ _ _ _ TS).
     constructor. by apply VAL.
-  - punfold SIM. destruct (SIM WFS WFT SIM0) as (SU & DIV & ?); [naive_solver|].
+  - punfold SIM. destruct (SIM WFS WFT) as [SU]; [naive_solver|].
     destruct SU as (eσ2 & TS' & IN & NR).
     + split; [by apply expr_terminal_False|].
       intros ???? PRIM. eapply (NS (e', σ')). econstructor; eauto.
     + apply (rtc_step_behavior _ _ _ _ TS').
       constructor 2; [by apply expr_terminal_False|].
       intros ? RED. inversion RED. by apply (NR _ _ _ _ PRIM).
-  - punfold SIM. destruct (SIM WFS WFT SIM0) as (SU & DIV & ?); [naive_solver|].
-    constructor. by apply DIV.
+  (* - punfold SIM. destruct (SIM WFS WFT SIM0) as (SU & DIV & ?); [naive_solver|].
+    constructor. by apply DIV. *)
   - punfold SIM.
-    destruct (SIM WFS WFT SIM0) as (SU & DIV & TERM & TS); [naive_solver|].
-    destruct (TS cfg_tgt' STEP) as (eσ & σG' & STEP' & SS & HΦ & TS').
+    destruct (SIM WFS WFT) as [SU (* DIV *) TERM TS]; [naive_solver|].
+    destruct (TS cfg_tgt' STEP) as (eσ & STEP' & TS').
     eapply rtc_step_behavior; first by apply STEP'.
     eapply IH; simpl.
     + by apply (rtc_tstep_wf _ _ STEP').
     + by apply (tstep_wf _ _ STEP).
-    + eauto.
-    + intros cfg' S'. apply NO_UB. by etrans.
+    + clear -STEP' NO_UB. induction STEP'. done.
+      apply IHSTEP'. admit.
     + by inversion TS'.
-Qed.
+Abort.
